theories/simplang/na_inv/readonly_refl.v
@@ -1,6 +1,6 @@
 From simuliris.simulation Require Import slsls lifting.
 From simuliris.simplang Require Import proofmode tactics.
-From simuliris.simplang Require Import parallel_subst gen_log_rel gen_refl pure_refl wf.
+From simuliris.simplang Require Import gen_log_rel gen_refl pure_refl wf.
 From simuliris.simplang.na_inv Require Export inv.
 From iris.prelude Require Import options.
 
