theories/simplang/simple_inv/refl.v
@@ -1,6 +1,6 @@
 From simuliris.simulation Require Import slsls lifting.
 From simuliris.simplang Require Import proofmode tactics.
-From simuliris.simplang Require Import parallel_subst gen_log_rel wf gen_refl pure_refl.
+From simuliris.simplang Require Import gen_log_rel wf gen_refl pure_refl.
 From simuliris.simplang.simple_inv Require Import inv.
 From iris.prelude Require Import options.
 
@@ -72,22 +72,6 @@ Section refl.
     log_rel e_t e_s -∗ log_rel (fill_ctx C e_t) (fill_ctx C e_s).
   Proof.
     intros ?. iApply gen_log_rel_ctx; first by apply simple_log_rel_structural. done.
-  Qed.
-
-  Corollary log_rel_ectx K e_t e_s :
-    ectx_wf K →
-    log_rel e_t e_s -∗ log_rel (fill K e_t) (fill K e_s).
-  Proof.
-    intros ?. iApply gen_log_rel_ectx; first by apply simple_log_rel_structural. done.
-  Qed.
-
-  Lemma log_rel_closed_1 e_t e_s π :
-    free_vars e_t ∪ free_vars e_s = ∅ →
-    log_rel e_t e_s ⊢ e_t ⪯{π} e_s {{ λ v_t v_s, val_rel v_t v_s }}.
-  Proof.
-    iIntros (?) "#Hrel".
-    iApply sim_mono; last iApply (gen_log_rel_closed_1 with "Hrel"); [|done..].
-    iIntros (v_t v_s) "[_ $]".
   Qed.
 
 End refl.
