theories/simulation/slsls.v
@@ -127,7 +127,7 @@ Section fix_lang.
         ⌜e_t = fill K_t (of_call f v_t)⌝ ∗
         ⌜no_forks P_s e_s σ_s (fill K_s' (of_call f v_s)) σ_s'⌝ ∗
         ext_rel π v_t v_s ∗ state_interp P_t σ_t P_s σ_s' (<[π := fill K_s (fill K_s' (of_call f v_s))]> T_s) ∗
-        (∀ v_t v_s, ext_rel π  v_t v_s -∗ greatest_rec Φ π (fill K_t (of_val v_t)) (fill K_s' (of_val v_s)) ))
+        (∀ v_t v_s, ext_rel π v_t v_s -∗ greatest_rec Φ π (fill K_t (of_val v_t)) (fill K_s' (of_val v_s)) ))
     )%I.
 
 
@@ -349,6 +349,7 @@ Section fix_lang.
     rewrite /sim_expr_ectx sim_expr_fixpoint /sim_expr_inner //.
   Qed.
 
+  (* FIXME: should use [pointwise_relation] *)
   Global Instance sim_expr_ne:
     NonExpansive4 (sim_expr: expr_rel → thread_id → expr_rel).
   Proof. rewrite sim_expr_eq. apply _. Qed.
@@ -360,6 +361,20 @@ Section fix_lang.
     rewrite !sim_expr_eq. eapply greatest_def_proper; done.
   Qed.
 
+  (* FIXME: should use [pointwise_relation] *)
+  Global Instance sim_ne:
+    NonExpansive4 (sim: (val Λ -d> val Λ -d> PROP) → thread_id → expr_rel).
+  Proof.
+    intros ? ?? Hpost ??? ??? ???. apply sim_expr_ne; [|done..].
+    rewrite /lift_post => ??. repeat f_equiv. apply Hpost.
+  Qed.
+
+  Global Instance sim_proper:
+    Proper ((pointwise_relation (val Λ) (pointwise_relation (val Λ) (≡))) ==> eq ==> eq ==> eq ==> (≡)) (sim).
+  Proof.
+    intros ?? Hpost ??? ??? ???. apply sim_expr_proper; [|done..].
+    rewrite /lift_post => ??. repeat f_equiv.
+  Qed.
 
   Existing Instances least_def_body_mono greatest_def_body_mono.
   (* any post-fixed point is included in the gfp *)
@@ -758,12 +773,16 @@ Section fix_lang.
   Qed.
 
   (** Corollaries *)
-  Lemma sim_call_inline P_t P_s v_t v_s K_t K_s f Φ π :
-    P_t !! f = Some K_t →
-    P_s !! f = Some K_s →
-    ⊢ progs_are P_t P_s ∗ ext_rel π v_t v_s ∗ sim_expr_ectx π K_t K_s Φ -∗ (of_call f v_t) ⪯{π} (of_call f v_s) [{ Φ }].
+  Lemma sim_call_inline P_t P_s v_t v_s x_t x_s e_f_t e_f_s f Φ π :
+    P_t !! f = Some (x_t, e_f_t) →
+    P_s !! f = Some (x_s, e_f_s) →
+    ⊢ progs_are P_t P_s -∗
+      ext_rel π v_t v_s -∗
+      (∀ v'_t v'_s, ext_rel π v'_t v'_s -∗
+        (subst_map {[x_t:=v'_t]} e_f_t) ⪯{π} (subst_map {[x_s:=v'_s]} e_f_s) [{ Φ }]) -∗
+      (of_call f v_t) ⪯{π} (of_call f v_s) [{ Φ }].
  Proof.
-    intros Htgt Hsrc. iIntros "(#Prog & Val & Sim)".
+    intros Htgt Hsrc. iIntros "#Prog Val Sim".
     rewrite sim_expr_unfold. iIntros (P_t' σ_t P_s' σ_s T_s K_s') "[SI [% %]]".
     iModIntro. iRight. iLeft.
     rewrite /progs_are; iDestruct ("Prog" with "SI") as "[% %]"; subst P_t' P_s'; iClear "Prog".
@@ -771,7 +790,7 @@ Section fix_lang.
     - iPureIntro. eapply head_prim_reducible. eexists _, _, _.
       by eapply call_head_step_intro.
     - iIntros (e_t' efs σ_t' Hstep). iModIntro.
-      pose proof (prim_step_call_inv P_t empty_ectx f v_t e_t' σ_t σ_t' efs) as (K_t' & Heq & -> & -> & ->);
+      pose proof (prim_step_call_inv P_t empty_ectx f v_t e_t' σ_t σ_t' efs) as (x_t' & e_f_t' & Heq & -> & -> & ->);
         first by rewrite fill_empty.
       rewrite fill_empty in Hstep. iRight.
       iExists _, _, _, _, _. iSplit; last iSplit; last iSplit; last iSplitL "SI".
@@ -780,7 +799,8 @@ Section fix_lang.
       + done.
       + rewrite app_nil_r. iApply (state_interp_pure_prim_step with "SI"); [done|]. intros ?.
         eapply fill_prim_step. eapply head_prim_step, call_head_step_intro, Hsrc.
-      + rewrite fill_empty; assert (K_t' = K_t) as -> by naive_solver.
+      + rewrite fill_empty. assert (x_t' = x_t) as -> by naive_solver.
+        assert (e_f_t' = e_f_t) as -> by naive_solver.
         iSpecialize ("Sim" with "Val"). simpl. iFrame.
   Qed.
 
